Blanc/ReCommonTest.lean
@@ -1,0 +1,3 @@
+import Blanc.ReCommon
+open List
+#check List.drop_zero
